lean/Hourglass.lean
@@ -1,4 +1,5 @@
 import Hourglass.Funs
 import Hourglass.FunsExternal
 import Hourglass.Laws
+import Hourglass.Merge
 import Hourglass.Trust
